src/Norm.v
@@ -18,7 +18,7 @@ Import ListNotations.
 Definition normal_form {X : Type} (R : relation X) (t : X) : Prop :=
   ¬ ∃ t', R t t'.
 
-Theorem value_is_nf {τ} (v : Exp [] τ) :
+Theorem value_is_nf {Γ τ} (v : Exp Γ τ) :
   ValueP v → normal_form Step v.
 Proof.
   intros.
@@ -39,30 +39,31 @@ Ltac normality :=
         now exists Y
   end.
 
-Lemma If_loop_true {τ} b {x : Exp [] τ} {y : Exp [] τ} :
+Lemma If_loop_true {Γ τ} b {x : Exp Γ τ} {y : Exp Γ τ} :
   ¬ (If b x y = x).
 Proof.
   induction x; intro; inv H.
   now eapply IHx2; eauto.
 Qed.
 
-Lemma If_loop_false {τ} b {x : Exp [] τ} {y : Exp [] τ} :
+Lemma If_loop_false {Γ τ} b {x : Exp Γ τ} {y : Exp Γ τ} :
   ¬ (If b x y = y).
 Proof.
   induction y; intro; inv H.
   now eapply IHy3; eauto.
 Qed.
 
-Lemma Seq_loop {τ ty} {x : Exp [] ty} {y : Exp [] τ} :
+Lemma Seq_loop {Γ τ ty} {x : Exp Γ ty} {y : Exp Γ τ} :
   ¬ (Seq x y = y).
 Proof.
   induction y; intro; inv H.
   now eapply IHy2; eauto.
 Qed.
 
-Lemma Let_loop {τ ty} {v : Exp [] ty} {e : Exp [ty ] τ} :
+Lemma Let_loop {Γ τ ty} {v : Exp Γ ty} {e : Exp (ty :: Γ) τ} :
   ¬ (STmExp {||v||} e = Let v e).
 Proof.
+  generalize dependent Γ.
   dependent induction e; repeat intro; inv H.
   - admit.
   - dependent induction v0; simp consSub in *.
@@ -70,7 +71,7 @@ Proof.
     + now induction v0; inv H1; intuition.
 Admitted.
 
-Lemma App_Lam_loop {τ ty} {v : Exp [] ty} {e : Exp [ty ] τ} :
+Lemma App_Lam_loop {Γ τ ty} {v : Exp Γ ty} {e : Exp (ty :: Γ) τ} :
   ¬ (STmExp {||v||} e = APP (LAM e) v).
 Proof.
   dependent induction e; repeat intro; inv H.
@@ -81,7 +82,7 @@ Proof.
 Admitted.
 
 (* A term never reduces to itself. *)
-Theorem Step_irr {τ} {x : Exp [] τ} : ¬ (x ---> x).
+Theorem Step_irr {Γ τ} {x : Exp Γ τ} : ¬ (x ---> x).
 Proof.
   intro.
   dependent induction x; try solve [ now inv H ].
@@ -89,15 +90,6 @@ Proof.
     + now eapply If_loop_true; eauto.
     + now eapply If_loop_false; eauto.
     + now firstorder.
-  - inv H.
-    + now eapply IHx1; eauto.
-    + now eapply IHx2; eauto.
-  - inv H.
-    + now eapply IHx; eauto.
-    + now eapply IHx; eauto.
-  - inv H.
-    + now eapply IHx; eauto.
-    + now eapply IHx; eauto.
   - inv H.
     now eapply Seq_loop; eauto.
   - inv H.
@@ -109,7 +101,7 @@ Proof.
     + now eapply IHx2; eauto.
 Qed.
 
-Corollary Step_productive {τ} {x x' : Exp [] τ} : x ---> x' → x ≠ x'.
+Corollary Step_productive {Γ τ} {x x' : Exp Γ τ} : x ---> x' → x ≠ x'.
 Proof.
   repeat intro; subst.
   now eapply Step_irr; eauto.
@@ -117,16 +109,16 @@ Qed.
 
 (* This injectivity theorem says that there is exactly one way to reduce terms
    at any given step. *)
-Fixpoint Step_inj {τ} {x y z : Exp [] τ} :
+Fixpoint Step_inj {Γ τ} {x y z : Exp Γ τ} :
   x ---> y → x ---> z → y = z.
 Proof.
   intros.
   dependent induction x; intros; try solve [ now inv H ].
   - inv H; inv H0; auto.
-    + now inv H2.
-    + now inv H2.
     + now inv H3.
     + now inv H3.
+    + now inv H4.
+    + now inv H4.
     + now f_equal; intuition.
   - inv H; inv H0; auto.
     + now f_equal; intuition.
@@ -135,18 +127,18 @@ Proof.
     + now f_equal; intuition.
   - inv H; inv H0; auto.
     + now f_equal; intuition.
+    + now inv H4; normality.
     + now inv H3; normality.
-    + now inv H2; normality.
   - inv H; inv H0; auto.
     + now f_equal; intuition.
+    + now inv H4; normality.
     + now inv H3; normality.
-    + now inv H2; normality.
   - now inv H; inv H0.
   - inv H; inv H0; auto.
     + now f_equal; intuition.
     + now normality.
     + now normality.
-  - inv H; inv H0; auto; try solve [ now inv H2 ].
+  - inv H; inv H0; auto; try solve [ now inv H3 ].
     + now normality.
     + now f_equal; intuition.
     + now normality.
@@ -157,22 +149,22 @@ Qed.
 Definition deterministic {X : Type} (R : relation X) :=
   ∀ x y1 y2 : X, R x y1 → R x y2 → y1 = y2.
 
-Theorem step_deterministic τ :
-  deterministic (@Step τ).
+Theorem step_deterministic Γ τ :
+  deterministic (@Step Γ τ).
 Proof.
   repeat intro.
   generalize dependent y2.
   dependent induction x; intros; inv H.
   (* ST_IfTrue *)
   - inv H0; auto.
-    now inv H2.
+    now inv H3.
   (* ST_IfFalse *)
   - inv H0; auto.
-    now inv H2.
+    now inv H3.
   (* ST_If *)
   - inv H0.
-    + now inv H3.
-    + now inv H3.
+    + now inv H4.
+    + now inv H4.
     + now f_equal; intuition.
   (* ST_Pair1 *)
   - inv H0.
@@ -186,18 +178,18 @@ Proof.
   - inv H0.
     + now f_equal; intuition.
     + exfalso.
-      now inv H3; normality.
+      now inv H4; normality.
   (* ST_FstPair *)
   - inv H0; auto.
-    now inv H2; normality.
+    now inv H3; normality.
   (* ST_Snd1 *)
   - inv H0.
     + now f_equal; intuition.
     + exfalso.
-      now inv H3; normality.
+      now inv H4; normality.
   (* ST_SndPair *)
   - inv H0; auto.
-    now inv H2; normality.
+    now inv H3; normality.
   (* ST_Seq *)
   - inv H0.
     now intuition.
@@ -210,11 +202,11 @@ Proof.
     now normality.
   (* ST_AppAbs *)
   - inv H0; auto.
-    + now inv H2.
+    + now inv H3.
     + now normality.
   (* ST_App1 *)
   - inv H0.
-    + now inv H3.
+    + now inv H4.
     + now f_equal; intuition.
     + now normality.
   (* ST_App2 *)
@@ -291,7 +283,7 @@ Proof.
         now constructor.
 Qed.
 
-Corollary nf_is_value τ (v : Exp [] τ) :
+Corollary nf_is_value {τ} (v : Exp [] τ) :
   normal_form Step v → ValueP v.
 Proof.
   intros.
@@ -300,7 +292,7 @@ Proof.
   now apply H.
 Qed.
 
-Corollary nf_same_as_value τ (v : Exp [] τ) :
+Corollary nf_same_as_value {τ} (v : Exp [] τ) :
   normal_form Step v ↔ ValueP v.
 Proof.
   split.
@@ -335,17 +327,17 @@ Proof.
   now eapply multi_step; eauto.
 Qed.
 
-Definition halts {τ} (e : Exp [] τ) : Prop :=
+Definition halts {Γ τ} (e : Exp Γ τ) : Prop :=
   ∃ e', e --->* e' ∧ ValueP e'.
 
-Lemma value_halts {τ} (v : Exp [] τ) : ValueP v → halts v.
+Lemma value_halts {Γ τ} (v : Exp Γ τ) : ValueP v → halts v.
 Proof.
   intros.
   unfold halts.
   now dependent induction H; eexists; split; constructor.
 Qed.
 
-Lemma step_preserves_halting {τ} (e e' : Exp [] τ) :
+Lemma step_preserves_halting {Γ τ} (e e' : Exp Γ τ) :
   (e ---> e') → (halts e ↔ halts e').
 Proof.
   intros.
@@ -356,7 +348,7 @@ Proof.
     + apply value_is_nf in H2.
       destruct H2.
       now exists e'.
-    + rewrite (step_deterministic _ _ _ _ H H0).
+    + rewrite (step_deterministic _ _ _ _ _ H H0).
       now exists z.
   - intros [e'0 [H1 H2]].
     exists e'0.
@@ -364,11 +356,11 @@ Proof.
     now eapply multi_step; eauto.
 Qed.
 
-Definition normal_form_of {τ} (e e' : Exp [] τ) :=
+Definition normal_form_of {Γ τ} (e e' : Exp Γ τ) :=
   (e --->* e' ∧ normal_form Step e').
 
-Theorem normal_forms_unique τ :
-  deterministic (normal_form_of (τ:=τ)).
+Theorem normal_forms_unique Γ τ :
+  deterministic (normal_form_of (Γ:=Γ) (τ:=τ)).
 Proof.
   unfold deterministic, normal_form_of.
   intros x y1 y2 P1 P2.
@@ -389,3 +381,129 @@ Qed.
 
 Definition normalizing {X : Type} (R : relation X) :=
   ∀ t, ∃ t', (multi R) t t' ∧ normal_form R t'.
+
+Equations R {Γ τ} (e : Γ ⊢ τ) : Prop :=
+  R (τ:=TyPrim _) e := halts e;
+  R (τ:=TyUnit)   e := halts e;
+  R (τ:=TyBool)   e := halts e;
+  R (τ:=_ × _)    e := halts e ∧ R (Fst e) ∧ R (Snd e);
+  R (τ:=_ ⟶ _)   e := halts e ∧ ∀ e', R e' → R (APP e e').
+
+Lemma R_halts {Γ τ} {e : Γ ⊢ τ} : R e → halts e.
+Proof. intros; induction τ; simp R in H; now reduce. Qed.
+
+Lemma step_preserves_R {Γ τ} {e e' : Γ ⊢ τ} :
+  (e ---> e') → R e → R e'.
+Proof.
+  intros.
+  induction τ; simp R in *;
+  pose proof H as H1;
+  apply step_preserves_halting in H1; intuition.
+  - eapply IHτ1; eauto.
+    now constructor.
+  - eapply IHτ2; eauto.
+    now constructor.
+  - eapply IHτ2; eauto.
+    now constructor.
+Qed.
+
+Lemma multistep_preserves_R {Γ τ} {e e' : Γ ⊢ τ} :
+  (e --->* e') → R e → R e'.
+Proof.
+  intros.
+  induction H; auto.
+  apply IHmulti.
+  now eapply step_preserves_R; eauto.
+Qed.
+
+Lemma step_preserves_R' {Γ τ} {e e' : Γ ⊢ τ} :
+  (e ---> e') → R e' → R e.
+Proof.
+  intros.
+  induction τ; simp R in *;
+  pose proof H as H1;
+  apply step_preserves_halting in H1; intuition.
+  - eapply IHτ1; eauto.
+    now constructor.
+  - eapply IHτ2; eauto.
+    now constructor.
+  - eapply IHτ2; eauto.
+    now constructor.
+Qed.
+
+Lemma multistep_preserves_R' {Γ τ} {e e' : Γ ⊢ τ} :
+  (e --->* e') → R e' → R e.
+Proof.
+  intros.
+  induction H; auto.
+  now eapply step_preserves_R'; eauto.
+Qed.
+
+Inductive ExpEnv : Env → Type :=
+  | Nil : ExpEnv []
+  | Cons {Γ τ} : Exp Γ τ → ExpEnv Γ →  ExpEnv (τ :: Γ).
+
+Equations msubst `(e : Γ ⊢ τ) `(ss : ExpEnv Γ) : [] ⊢ τ :=
+  msubst (Γ:=[]) e Nil => e;
+  msubst e (Cons x xs) => msubst (STmExp {|| x ||} _) xs.
+
+Definition mupdate := app.
+
+Lemma msubst_closed `(e : [] ⊢ τ) ss :
+  msubst e ss = e.
+Proof.
+  dependent induction ss.
+  now simp msubst.
+Qed.
+
+Inductive instantiation : ∀ Γ, ExpEnv Γ → Prop :=
+  | V_nil :
+      instantiation [] Nil
+  | V_cons {Γ τ} (v : Γ ⊢ τ) ee :
+      ValueP v → R v →
+      instantiation Γ ee →
+      instantiation (τ :: Γ) (Cons v ee).
+
+Lemma multistep_App2 {Γ dom cod} {e e' : Γ ⊢ dom} {v : Γ ⊢ (dom ⟶ cod)} :
+  ValueP v → (e --->* e') → APP v e --->* APP v e'.
+Proof.
+  intros.
+  induction H0.
+  - now apply multi_refl.
+  - eapply multi_step; eauto.
+    now constructor.
+Qed.
+
+(* Equations ExpGet `(se : ExpEnv Γ) `(v : Var Γ τ) : Γ ⊢ τ := *)
+(*   ExpGet (Cons x _)   ZV    := x; *)
+(*   ExpGet (Cons _ xs) (SV v) := ExpGet xs v. *)
+
+Lemma msubst_R : ∀ Γ (env : ExpEnv Γ) τ (t : Exp Γ τ),
+  instantiation Γ env →
+  R (msubst t env).
+Proof.
+  intros Γ env τ t V.
+  generalize dependent env.
+  (* We need to generalize the hypothesis a bit before setting up the induction. *)
+  generalize dependent Γ.
+  induction t; intros.
+  - admit.
+  - admit.
+  - admit.
+  - admit.
+  - admit.
+  - admit.
+  - admit.
+  - admit.
+  - admit.
+  - admit.
+  (* - apply instantiation_R. *)
+Admitted.
+
+Theorem normalization {τ} (e : [] ⊢ τ) : halts e.
+Proof.
+  replace e with (msubst e Nil) by reflexivity.
+  apply R_halts.
+  apply (msubst_R nil); eauto.
+  now constructor.
+Qed.
