src/Sub.v
@@ -1,5 +1,5 @@
 Require Export
-  Coq.micromega.Lia
+  Coq.Program.Equality
   Ty
   Exp
   Ren.
@@ -25,11 +25,35 @@ Definition tlSub {Γ Γ' τ} (s : Sub (τ :: Γ) Γ') : Sub Γ Γ' :=
   fun τ' v => s τ' (SV v).
 Definition hdSub {Γ Γ' τ} (s : Sub (τ :: Γ) Γ') : Exp Γ' τ := s τ ZV.
 
+Definition sskip1 {Γ τ} : Sub Γ (τ :: Γ) := λ _ v, VAR (SV v).
+
 Equations STmL {Γ Γ' τ} (s : Sub Γ Γ')
           (* Sub (τ :: Γ) (τ :: Γ') *)
           τ' (v : Var (τ :: Γ) τ') : Exp (τ :: Γ') τ' :=
   STmL _ τ' ZV      := VAR ZV;
   STmL _ τ' (SV v') := wk (s _ v').
+
+Lemma STmL_idSub {Γ τ} : @STmL Γ Γ τ idSub = idSub.
+Proof.
+  extensionality τ'.
+  extensionality v.
+  dependent elimination v.
+  - now rewrite STmL_equation_1.
+  - now rewrite STmL_equation_2.
+Qed.
+
+Corollary tlSub_idSub {Γ τ} : @tlSub Γ _ τ idSub = sskip1.
+Proof. reflexivity. Qed.
+
+Notation "{|| e ; .. ; f ||}" := (consSub e .. (consSub f idSub) ..).
+
+Lemma tlSub_sing Γ τ (x : Exp Γ τ) : tlSub {|| x ||} = idSub.
+Proof.
+  unfold tlSub, idSub.
+  extensionality τ'.
+  extensionality v.
+  now induction v; simp consSub.
+Qed.
 
 Fixpoint STmExp {Γ Γ' τ} (s : Sub Γ Γ') (e : Exp Γ τ) : Exp Γ' τ :=
   match e with
@@ -49,13 +73,103 @@ Fixpoint STmExp {Γ Γ' τ} (s : Sub Γ Γ') (e : Exp Γ τ) : Exp Γ' τ :=
   | LAM e         => LAM (STmExp (STmL s) e)
   end.
 
+Ltac Rewrites E :=
+  (intros; simpl; try rewrite E;
+   repeat match goal with
+          | [H : _ = _ |- _ ] => rewrite H; clear H
+          end; auto).
+
+Lemma STmExp_idSub {Γ τ} (e : Exp Γ τ) :
+  STmExp idSub e = e.
+Proof.
+  induction e; simpl; auto;
+  now Rewrites (@STmL_idSub Γ).
+Qed.
+
+Definition ScS {Γ Γ' Γ''} (s : Sub Γ' Γ'') (s' : Sub Γ Γ') :=
+  (λ τ v, STmExp s (s' τ v)) : Sub Γ Γ''.
+
+Corollary tlSub_sskip1 Γ Γ' τ (f : Sub (τ :: Γ') Γ) :
+  tlSub f = ScS f sskip1.
+Proof. reflexivity. Qed.
+
+Corollary ScS_idSub_left Γ Γ' (f : Sub Γ' Γ) :
+  ScS idSub f = f.
+Proof.
+  unfold ScS.
+  extensionality τ.
+  extensionality v.
+  now rewrite STmExp_idSub.
+Qed.
+
+Corollary ScS_idSub_right Γ Γ' (f : Sub Γ' Γ) :
+  ScS f idSub = f.
+Proof.
+  unfold ScS.
+  extensionality τ.
+  extensionality v.
+  now induction v.
+Qed.
+
+Corollary ScS_assoc Γ Γ' Γ'' Γ'''
+          (f : Sub Γ' Γ) (g : Sub Γ'' Γ') (h : Sub Γ''' Γ'') :
+  ScS f (ScS g h) = ScS (ScS f g) h.
+Proof.
+  unfold ScS.
+  extensionality τ.
+  extensionality v.
+  induction (h τ v); simpl; auto;
+  rewrite ?STmL_idSub, ?IHe1, ?IHe2, ?IHe3, ?IHe; auto.
+Abort.
+
 Definition ScR {Γ Γ' Γ''} (s : Sub Γ' Γ'') (r : Ren Γ Γ') :=
   (λ τ v, s τ (r τ v)) : Sub Γ Γ''.
 
 Definition RcS {Γ Γ' Γ''} (r : Ren Γ' Γ'') (s : Sub Γ Γ') :=
   (λ τ v, RTmExp r (s τ v)) : Sub Γ Γ''.
 
-Definition ScS {Γ Γ' Γ''} (s : Sub Γ' Γ'') (s' : Sub Γ Γ') :=
-  (λ τ v, STmExp s (s' τ v)) : Sub Γ Γ''.
+Lemma LiftScR {Γ Γ' Γ'' τ} (r : Ren Γ Γ') (s : Sub Γ' Γ'') :
+  STmL (τ:=τ) (ScR s r) = ScR (STmL s) (RTmL r).
+Proof.
+Admitted.
 
-Notation "{|| e ; .. ; f ||}" := (consSub e .. (consSub f idSub) ..).
+Lemma ActionScR {Γ Γ' Γ'' τ} (r : Ren Γ Γ') (s : Sub Γ' Γ'') (e : Exp Γ τ) :
+  STmExp (ScR s r) e = STmExp s (RTmExp r e).
+Proof.
+Admitted.
+
+Lemma LiftRcS {Γ Γ' Γ'' τ} (r : Ren Γ' Γ'') (s : Sub Γ Γ') :
+  STmL (τ:=τ) (RcS r s) = RcS (RTmL r) (STmL s).
+Proof.
+Admitted.
+
+Lemma ActionRcS {Γ Γ' Γ'' τ} (r : Ren Γ' Γ'') (s : Sub Γ Γ') (e : Exp Γ τ) :
+  STmExp (RcS r s) e = RTmExp r (STmExp s e).
+Proof.
+Admitted.
+
+Lemma LiftScS {Γ Γ' Γ'' τ} (s : Sub Γ' Γ'') (s' : Sub Γ Γ') :
+  STmL (τ:=τ) (ScS s s') = ScS (STmL s) (STmL s').
+Proof.
+  extensionality τ'.
+  extensionality v.
+  unfold ScS.
+  dependent induction v.
+  - now simp STmL; simpl; simp STmL.
+  - simp STmL; simpl; simp STmL.
+    unfold wk.
+    now rewrite <- ActionRcS, <- ActionScR.
+Qed.
+
+Lemma ActionScS {Γ Γ' Γ'' τ} (s : Sub Γ' Γ'') (s' : Sub Γ Γ') (e : Exp Γ τ) :
+  STmExp (ScS s s') e = STmExp s (STmExp s' e).
+Proof.
+  generalize dependent Γ''.
+  generalize dependent Γ'.
+  induction e; simpl; intros; auto;
+  rewrite ?STmL_idSub, ?IHe1, ?IHe2, ?IHe3, ?IHe; auto.
+  - rewrite LiftScS.
+    now rewrite IHe2.
+  - rewrite LiftScS.
+    now rewrite IHe.
+Qed.
